SecurityNotation/Testing/testing_initialKnowledge.lean
@@ -4,11 +4,13 @@ import SecurityNotation.Basic.Syntax.Principal
 import SecurityNotation.Basic.Syntax.Keys
 import SecurityNotation.Basic.Syntax.Messages
 
-def Alice : Principal := {id := 1, name := "Alice", role := Role.initiator}
-def Bob : Principal := {id := 2, name := "Bob", role := Role.responder}
+def Alice : Principal := {id := 1, name := "Alice", role := Role.initiator, known_principals := []}
+def Bob : Principal := {id := 2, name := "Bob", role := Role.responder, known_principals := []}
 
 def Bob_pub  : Key := Key.new 1 keyType.publicKey  (some Bob) []
 def Bob_priv : Key := Key.new 2 keyType.privateKey (some Bob) []
 def session  : Key := Key.new 3 keyType.sessionKey  none      [Alice, Bob]
 
- 
+-- testing that alice knows of bob if stated in initial knowledge
+example : Initial_knowledge Alice (Message.agent Bob) :=
+  Initial_knowledge.knows_agents Bob
