SecurityNotation/Testing/testing_trace.lean
@@ -1,9 +1,0 @@
-import SecurityNotation.Basic.Syntax.Principal
-import SecurityNotation.Basic.Syntax.Nonces
-import SecurityNotation.Basic.Syntax.Keys
-import SecurityNotation.Basic.Syntax.Messages
-import SecurityNotation.Basic.Syntax.Events
-import SecurityNotation.Logic.Logic
-
--- testing trace and event
-
